Strata/DL/Lambda/LExpr.lean
@@ -506,6 +506,7 @@ def size (T : LExprParamsT) (e : LExpr T) : Nat :=
 Erase all type annotations from `e` except the bound variables of abstractions
 and quantified expressions.
 -/
+@[expose]
 def eraseTypes {T : LExprParamsT} (e : LExpr T) : LExpr T :=
   match e with
   | .const m c => .const m c
@@ -513,7 +514,7 @@ def eraseTypes {T : LExprParamsT} (e : LExpr T) : LExpr T :=
   | .fvar m x _ => .fvar m x none
   | .bvar _ _ => e
   | .abs m name ty e => .abs m name ty (eraseTypes e)
-  | .quant m qk name _ tr e => .quant m qk name .none (eraseTypes tr) (eraseTypes e)
+  | .quant m qk name ty tr e => .quant m qk name ty (eraseTypes tr) (eraseTypes e)
   | .app m e1 e2 => .app m (eraseTypes e1) (eraseTypes e2)
   | .ite m c t f => .ite m (eraseTypes c) (eraseTypes t) (eraseTypes f)
   | .eq m e1 e2 => .eq m (eraseTypes e1) (eraseTypes e2)
